theories/Decidability/UntypedCompleteness.v
@@ -1,0 +1,355 @@
+(** * LogRel.Decidability.UntypedCompleteness: the inductive predicates imply the implementation answer positively. *)
+From Coq Require Import Nat Lia Arith.
+From Equations Require Import Equations.
+From LogRel.AutoSubst Require Import core unscoped Ast Extra.
+From LogRel Require Import BasicAst Context Notations UntypedReduction DeclarativeTyping DeclarativeInstance GenericTyping NormalForms.
+From LogRel Require Import Validity LogicalRelation Fundamental DeclarativeSubst TypeConstructorsInj AlgorithmicTyping BundledAlgorithmicTyping Normalisation AlgorithmicConvProperties AlgorithmicTypingProperties.
+From LogRel Require Import UntypedAlgorithmicConversion.
+From LogRel Require Import Utils. (* at the end, to get the right easy tactic… *)
+From LogRel.Decidability Require Import Functions UntypedFunctions Soundness UntypedSoundness Completeness.
+From PartialFun Require Import Monad PartialFun MonadExn.
+
+Set Universe Polymorphism.
+
+Import DeclarativeTypingProperties.
+
+Section ConversionComplete.
+
+Let PEq (t u : term) :=
+  (forall Γ, [Γ |-[de] t] × [Γ |-[de] u] -> graph _uconv (tm_state,t,u) ok) ×
+  (forall Γ A, [Γ |-[de] t : A] × [Γ |-[de] u : A] -> graph _uconv (tm_state,t,u) ok).
+
+Let PRedEq (t u : term) :=
+  (forall Γ, [Γ |-[de] t] × [Γ |-[de] u] -> graph _uconv (tm_red_state,t,u) ok) ×
+  (forall Γ A, isType A ->
+    [Γ |-[de] t : A] × [Γ |-[de] u : A] -> graph _uconv (tm_red_state,t,u) ok).
+
+Let PNeEq (t u : term) :=
+  forall Γ, well_typed Γ t × well_typed Γ u ->
+  graph _uconv (ne_state,t,u) ok.
+
+Ltac split_tm :=
+  split ;
+  [ intros * [Hz%type_isType Hz'%type_isType] ;
+    [solve [inversion Hz ; inv_whne | inversion Hz' ; inv_whne] | ..] ; now constructor
+  |..].
+
+Lemma uconv_complete :
+  UAlgoConvInductionConcl PEq PRedEq PNeEq.
+Proof.
+  subst PEq PRedEq PNeEq.
+  unfold UAlgoConvInductionConcl.
+  apply UAlgoConvInduction.
+
+  - intros * Ht Hu []%algo_uconv_wh [Hty Htm].
+    split.
+    all: intros * [Hconcl []]%dup.
+    all: unfold graph.
+    all: simp _uconv uconv_tm ; cbn.
+    all: repeat (match goal with |- orec_graph _ _ _ => patch_rec_ret ; econstructor end) ; cbn.
+    1-2: now eapply wh_red_complete_whnf_ty ; eauto.
+    2-3: now eapply wh_red_complete_whnf_tm ; eauto.
+    * eapply typeConvRed_prem2 in Hconcl ; eauto.
+      now eapply Hty.
+    * assert [Γ |-[de] A] as [[? ? wh]%type_normalisation]%dup by boundary. 
+      eapply termConvRed_prem3 in Hconcl ; eauto.
+      1: eapply Htm ; tea.
+      eapply type_isType ; tea.
+      now eapply subject_reduction_raw_ty.
+
+  - split.
+    all: intros.
+    all: unfold graph.
+    all: simp _uconv uconv_tm_red ; cbn.
+    all: econstructor.
+
+  - intros * ? [IHA_ty IHA_tm] ? [IHB_ty IHB_tm].
+    split.
+
+    + intros ? [Hconcl]%dup.
+      unfold graph.
+      simp _uconv uconv_tm_red ; cbn.
+
+      eapply typePiCongAlg_prem0 in Hconcl as [Hpre0 []]%dup.
+      econstructor ; [now eapply IHA_ty|..] ; cbn.
+      eapply implem_uconv_graph, uconv_sound in IHA_ty as [Hpost0%algo_conv_sound _]; tea.
+      eapply typePiCongAlg_prem1 in Hpost0 ; eauto.
+      patch_rec_ret ; econstructor ; [now eapply IHB_ty|..].
+      now constructor.
+
+  + intros * ? [Hconcl [[Hty]%dup]]%dup.
+    unfold graph.
+    simp _uconv uconv_tm_red ; cbn.
+    eapply termGen' in Hty as (?&[->]&->%red_ty_compl_univ_l%redty_sound%red_whnf) ; tea.
+    2: gen_typing.
+
+    eapply termPiCongAlg_prem0 in Hconcl as [Hpre0 []]%dup.
+    econstructor ; [now eapply IHA_tm|..] ; cbn.
+    eapply implem_uconv_graph, uconv_sound in IHA_tm as [_ Hpost0%algo_conv_sound]; tea.
+    eapply termPiCongAlg_prem1 in Hpost0 ; eauto.
+    patch_rec_ret ; econstructor ; [now eapply IHB_tm|..].
+    now constructor.
+
+  - split.
+    all: intros.
+    all: unfold graph.
+    all: simp _uconv uconv_tm_red build_nf_view2 ; cbn.
+    all: now constructor.
+
+  - split.
+    all: intros.
+    all: unfold graph.
+    all: simp _uconv uconv_tm_red build_nf_view2 ; cbn.
+    all: now constructor.
+
+  - intros * ? [_ IH_tm].
+    split_tm.
+    
+    intros ? T ? [[Hty] Hpre0]%dup.
+    unfold graph.
+    simp _uconv uconv_tm_red build_nf_view2 ; cbn.
+    eapply termGen' in Hty as (?&[->]&->%red_ty_compl_nat_l%redty_sound%red_whnf) ; tea.
+    2: gen_typing.
+    eapply termSuccCongAlg_prem0 in Hpre0.
+    patch_rec_ret ; econstructor ; [now eapply IH_tm|..].
+    now constructor.
+
+  - split.
+    all: intros.
+    all: unfold graph.
+    all: simp _uconv uconv_tm_red build_nf_view2 ; cbn.
+    all: now constructor.
+
+  - intros * ? [_ IH_tm].
+    split_tm.
+
+    intros * ? [Hconcl]%dup.
+    unfold graph.
+    simp _uconv uconv_tm_red build_nf_view2 ; cbn.
+    eapply LamCongUAlg_prem0 in Hconcl as (?&?&[->]); tea.
+    patch_rec_ret ; econstructor ; [now eapply IH_tm|..].
+    now constructor.
+
+  - intros * ? ? [_ IH_tm].
+    split_tm.
+
+    intros * ? [Hconcl]%dup.
+    unfold graph.
+    simp _uconv uconv_tm_red build_nf_view2.
+    unshelve erewrite whne_nf_view1 ; tea ; cbn.
+    eapply LamNeUAlg_prem0 in Hconcl as (?&?&[->]); tea.
+    patch_rec_ret ; econstructor ; [now eapply IH_tm|..].
+    now constructor.
+
+  - intros * ? ? [_ IH_tm].
+    split_tm.
+
+    intros * ? [Hconcl]%dup.
+    unfold graph.
+    simp _uconv uconv_tm_red build_nf_view2.
+    unshelve erewrite whne_nf_view1 ; tea ; cbn.
+    eapply NeLamUAlg_prem0 in Hconcl as (?&?&[->]); tea.
+    patch_rec_ret ; econstructor ; [now eapply IH_tm|..].
+    now constructor.
+
+  - intros * ? [IHA_ty IHA_tm] ? [IHB_ty IHB_tm].
+    split.
+
+    + intros ? [Hconcl]%dup.
+      unfold graph.
+      simp _uconv uconv_tm_red ; cbn.
+
+      eapply typeSigCongAlg_prem0 in Hconcl as [Hpre0 []]%dup.
+      econstructor ; [now eapply IHA_ty|..] ; cbn.
+      eapply implem_uconv_graph, uconv_sound in IHA_ty as [Hpost0%algo_conv_sound _]; tea.
+      eapply typeSigCongAlg_prem1 in Hpost0 ; eauto.
+      patch_rec_ret ; econstructor ; [now eapply IHB_ty|..].
+      now constructor.
+
+  + intros * ? [Hconcl [[Hty]%dup]]%dup.
+    unfold graph.
+    simp _uconv uconv_tm_red ; cbn.
+    eapply termGen' in Hty as (?&[->]&->%red_ty_compl_univ_l%redty_sound%red_whnf) ; tea.
+    2: gen_typing.
+
+    eapply termSigCongAlg_prem0 in Hconcl as [Hpre0 []]%dup.
+    econstructor ; [now eapply IHA_tm|..] ; cbn.
+    eapply implem_uconv_graph, uconv_sound in IHA_tm as [_ Hpost0%algo_conv_sound]; tea.
+    eapply termSigCongAlg_prem1 in Hpost0 ; eauto.
+    patch_rec_ret ; econstructor ; [now eapply IHB_tm|..].
+    now constructor.
+
+  - intros * ? [_ IHp] ? [_ IHq].
+    split_tm.
+    intros * ? [Hconcl [[Hty]%dup]]%dup.
+    unfold graph.
+    simp _uconv uconv_tm_red build_nf_view2 ; cbn.
+    eapply PairCongUAlg_prem0 in Hconcl as (?&?&[-> [Hpre0 []]%dup]) ; tea.
+    econstructor ; [now eapply IHp|..] ; cbn.
+    eapply implem_uconv_graph, uconv_sound in IHp as [_ Hpost0%algo_conv_sound]; tea.
+    eapply PairCongUAlg_prem1 in Hpost0 ; eauto.
+    patch_rec_ret ; econstructor ; [now eapply IHq|..].
+    now constructor.
+
+  - intros * ? ? [_ IHp] ? [_ IHq].
+    split_tm.
+    intros * ? [Hconcl [[Hty]%dup]]%dup.
+    unfold graph.
+    simp _uconv uconv_tm_red build_nf_view2 ; cbn.
+    unshelve erewrite whne_nf_view1 ; tea ; cbn.
+    eapply PairNeUAlg_prem0 in Hconcl as (?&?&[-> [Hpre0 []]%dup]) ; tea.
+    econstructor ; [now eapply IHp|..] ; cbn.
+    eapply implem_uconv_graph, uconv_sound in IHp as [_ Hpost0%algo_conv_sound]; tea.
+    eapply PairNeUAlg_prem1 in Hpost0 ; eauto.
+    patch_rec_ret ; econstructor ; [now eapply IHq|..].
+    now constructor.
+
+  - intros * ? ? [_ IHp] ? [_ IHq].
+    split_tm.
+    intros * ? [Hconcl [[Hty]%dup]]%dup.
+    unfold graph.
+    simp _uconv uconv_tm_red build_nf_view2 ; cbn.
+    unshelve erewrite whne_nf_view1 ; tea ; cbn.
+    eapply NePairUAlg_prem0 in Hconcl as (?&?&[-> [Hpre0 []]%dup]) ; tea.
+    econstructor ; [now eapply IHp|..] ; cbn.
+    eapply implem_uconv_graph, uconv_sound in IHp as [_ Hpost0%algo_conv_sound]; tea.
+    eapply NePairUAlg_prem1 in Hpost0 ; eauto.
+    patch_rec_ret ; econstructor ; [now eapply IHq|..].
+    now constructor.
+
+  - intros * ? [IHA_ty IHA_tm] ? [_ IHx] ? [_ IHy].
+    split.
+    
+    + intros ? [Hconcl]%dup.
+      unfold graph.
+      simp _uconv uconv_tm_red build_nf_view2 ; cbn.
+      eapply typeIdCongAlg_prem0 in Hconcl as [Hpre0 []]%dup.
+      econstructor ; [now eapply IHA_ty|..] ; cbn.
+      eapply implem_uconv_graph, uconv_sound in IHA_ty as [[Hpost0]%algo_conv_sound%dup _]; tea.
+      eapply typeIdCongAlg_prem1 in Hpost0 as [Hpre1 []]%dup ; eauto. 
+      econstructor ; [now eapply IHx|..] ; cbn.
+      eapply implem_uconv_graph, uconv_sound in IHx as [_ Hpost1%algo_conv_sound]; tea.
+      eapply typeIdCongAlg_prem2 in Hpost1 as [Hpre2 []]%dup ; eauto.
+      patch_rec_ret ; econstructor ; [now eapply IHy|..] ; cbn.
+      now econstructor.
+      
+    + intros ? ?? [Hconcl [[Hty]%dup]]%dup.
+      unfold graph.
+      simp _uconv uconv_tm_red build_nf_view2 ; cbn.
+      eapply termGen' in Hty as (?&[->]&->%red_ty_compl_univ_l%redty_sound%red_whnf) ; tea.
+      2: gen_typing.
+      eapply termIdCongAlg_prem0 in Hconcl as [Hpre0 []]%dup.
+      econstructor ; [now eapply IHA_tm|..] ; cbn.
+      eapply implem_uconv_graph, uconv_sound in IHA_tm as [_ [Hpost0]%algo_conv_sound%dup]; tea.
+      eapply termIdCongAlg_prem1 in Hpost0 as [Hpre1 []]%dup ; eauto. 
+      econstructor ; [now eapply IHx|..] ; cbn.
+      eapply implem_uconv_graph, uconv_sound in IHx as [_ Hpost1%algo_conv_sound]; tea.
+      eapply termIdCongAlg_prem2 in Hpost1 as [Hpre2 []]%dup ; eauto.
+      patch_rec_ret ; econstructor ; [now eapply IHy|..] ; cbn.
+      now econstructor.
+
+  - intros *.
+    split_tm.
+    intros.
+    unfold graph.
+    simp _uconv uconv_tm_red build_nf_view2 ; cbn.
+    econstructor.
+  
+  - intros * []%algo_uconv_wh IH.
+    split.
+
+    + intros ? Hconcl.
+      unfold graph.
+      simp _uconv uconv_tm_red build_nf_view2.
+      repeat (unshelve erewrite ! whne_nf_view1 ; tea ; cbn).
+      eapply typeNeuConvAlg_prem2 in Hconcl ; tea.
+      patch_rec_ret ; econstructor ; [now eapply IH|..] ; cbn.
+      now econstructor.
+
+    + intros ? ?? Hconcl.
+      unfold graph.
+      simp _uconv uconv_tm_red build_nf_view2.
+      repeat (unshelve erewrite ! whne_nf_view1 ; tea ; cbn).
+      eapply termNeuConvAlg_prem0 in Hconcl ; tea.
+      patch_rec_ret ; econstructor ; [now eapply IH|..] ; cbn.
+      now econstructor.
+
+  - intros.
+    unfold graph.
+    simp _uconv uconv_ne ; cbn.
+    rewrite Nat.eqb_refl ; cbn.
+    now econstructor.
+
+  - intros * ? IHm ? [_ IHt] ? [Hconcl]%dup.
+    unfold graph.
+    simp _uconv uconv_ne ; cbn.
+    eapply neuAppCongAlg_prem0 in Hconcl as [Hpre0 []]%dup ; eauto.
+    econstructor ; [now eapply IHm|..] ; cbn.
+    eapply implem_uconv_graph, uconv_sound in IHm as [? Hpost0] ; tea.
+    eapply AppCongUAlg_bridge in Hpost0 as (?&?&[? [Hpre1 []]%dup]); eauto.
+    eapply neuAppCongAlg_prem1 in Hpre1 as [Hpre1 []]%dup ; eauto. 
+    patch_rec_ret ; econstructor ; [now eapply IHt|..] ; cbn.
+    now constructor.
+
+  - intros * ? IH ? [IHP] ? [_ IHz] ? [_ IHs] ? [Hconcl]%dup.
+    unfold graph.
+    simp _uconv uconv_ne ; cbn.
+    eapply neuNatElimCong_prem0 in Hconcl as [Hpre0 []]%dup ; eauto.
+    econstructor ; [now eapply IH|..] ; cbn.
+    eapply implem_uconv_graph, uconv_sound in IH as [? Hpost0] ; tea.
+    eapply NatElimCongUAlg_bridge in Hpost0 as [? [Hpost0]%dup]; eauto.
+    eapply neuNatElimCong_prem1 in Hpost0 as [Hpre1 []]%dup ; eauto.
+    econstructor ; [now eapply IHP|..] ; cbn.
+    eapply implem_uconv_graph, uconv_sound in IHP as [Hpos1 _] ; tea.
+    eapply algo_conv_sound in Hpos1 as [Hpos1]%dup ; eauto.
+    eapply neuNatElimCong_prem2 in Hpos1 as [Hpre2 []]%dup ; eauto.
+    econstructor ; [now eapply IHz|..] ; cbn.
+    eapply implem_uconv_graph, uconv_sound in IHz as [_ Hpos2] ; tea.
+    eapply algo_conv_sound in Hpos2 as [Hpos2]%dup ; eauto.
+    eapply neuNatElimCong_prem3 in Hpos2 as [Hpre3 []]%dup ; eauto.
+    patch_rec_ret ; econstructor ; [now eapply IHs|..] ; cbn.
+    now constructor.
+    
+  - intros * ? IH ? [IHP] ? [Hconcl]%dup.
+    unfold graph.
+    simp _uconv uconv_ne ; cbn.
+    eapply neuEmptyElimCong_prem0 in Hconcl as [Hpre0 []]%dup ; eauto.
+    econstructor ; [now eapply IH|..] ; cbn.
+    eapply implem_uconv_graph, uconv_sound in IH as [? Hpost0] ; tea.
+    eapply EmptyElimCongUAlg_bridge in Hpost0 as [? [Hpost0]%dup]; eauto.
+    eapply neuEmptyElimCong_prem1 in Hpost0 as [Hpre1 []]%dup ; eauto.
+    patch_rec_ret ; econstructor ; [now eapply IHP|..] ; cbn.
+    now constructor.
+
+  - intros * ? IH ? [Hconcl]%dup.
+    unfold graph.
+    simp _uconv uconv_ne ; cbn.
+    eapply neuFstCongAlg_prem0 in Hconcl as [Hpre0 []]%dup ; eauto.
+    patch_rec_ret ; econstructor ; [now eapply IH|..] ; cbn.
+    now constructor.
+
+  - intros * ? IH ? [Hconcl]%dup.
+    unfold graph.
+    simp _uconv uconv_ne ; cbn.
+    eapply neuSndCongAlg_prem0 in Hconcl as [Hpre0 []]%dup ; eauto.
+    patch_rec_ret ; econstructor ; [now eapply IH|..] ; cbn.
+    now constructor.
+
+  - intros * ? IH ? [IHP] ? [_ IHe] ? [Hconcl]%dup.
+    unfold graph.
+    simp _uconv uconv_ne ; cbn.
+    eapply neuIdElimCong_prem0 in Hconcl as [Hpre0 []]%dup ; eauto.
+    econstructor ; [now eapply IH|..] ; cbn.
+    eapply implem_uconv_graph, uconv_sound in IH as [? Hpost0] ; tea.
+    eapply IdElimCongUAlg_bridge in Hpost0 as (?&?&?&[? [Hpost0]%dup]); eauto.
+    eapply neuIdElimCong_prem1 in Hpost0 as [Hpre1 []]%dup ; eauto.
+    econstructor ; [now eapply IHP|..] ; cbn.
+    eapply implem_uconv_graph, uconv_sound in IHP as [Hpos1 _] ; tea.
+    eapply algo_conv_sound in Hpos1 as [Hpos1]%dup ; eauto.
+    eapply neuIdElimCong_prem2 in Hpos1 as [Hpre2 []]%dup ; eauto.
+    patch_rec_ret ; econstructor ; [now eapply IHe|..] ; cbn.
+    now constructor.
+
+Qed.
+
+End ConversionComplete.
